rt abstract: spec for sporadic servers and period scheduling
See also SELFOUR-328 and SELFOUR-795

spec/abstract/SchedContext_A.thy
@@ -16,16 +16,278 @@ begin
 
 text \<open> This theory contains operations on scheduling contexts and scheduling control. \<close>
 
+definition "MIN_BUDGET = 2 * kernelWCET_ticks"
+definition "MIN_BUDGET_US = 2 * kernelWCET_us"
 
-text \<open> Replenish remaining time in scheduling context \<close>
+
 definition
-  recharge :: "obj_ref \<Rightarrow> (unit, 'z::state_ext) s_monad"
+  get_tcb_sc :: "obj_ref \<Rightarrow> (sched_context,'z::state_ext) s_monad" (* FIXME: RT - use this everywhere *)
 where
-  "recharge sc_ptr = do
+  "get_tcb_sc tcb_ptr = do
+    tcb \<leftarrow> gets_the $ get_tcb tcb_ptr;
+    sc_ptr \<leftarrow> assert_opt $ tcb_sched_context tcb;
+    get_sched_context sc_ptr
+  od"
+
+abbreviation
+  "refill_hd sc \<equiv> hd (sc_refills sc)"
+
+definition
+  get_sc_time :: "obj_ref \<Rightarrow> time det_ext_monad"
+where
+  "get_sc_time tcb_ptr = do
+    sc \<leftarrow> get_tcb_sc tcb_ptr;
+    return $ r_time (refill_hd sc)
+  od"
+
+
+text \<open>Enqueue a TCB in the release queue, sorted by release time of
+  the corresponding scheduling context.\<close>
+definition
+  tcb_release_enqueue :: "obj_ref \<Rightarrow> unit det_ext_monad"
+where
+  "tcb_release_enqueue tcb_ptr = do
+     time \<leftarrow> get_sc_time tcb_ptr;
+     qs \<leftarrow> gets release_queue;
+     times \<leftarrow> mapM get_sc_time qs;
+     qst \<leftarrow> return $ zip qs times;
+     qst' \<leftarrow> return $ filter (\<lambda>(_,t'). t' \<le> time) qst @ [(tcb_ptr,time)] @ filter (\<lambda>(_,t'). \<not>t' \<le> time) qst;
+     modify (\<lambda>s. s\<lparr>release_queue := map fst qst'\<rparr>)
+  od"
+
+definition
+  refills_capacity :: "time \<Rightarrow> refill list \<Rightarrow> time"
+where
+  "refills_capacity usage refills \<equiv>
+  if r_amount (hd refills) < usage then 0 else r_amount (hd refills) - usage"
+
+definition
+  get_refills :: "obj_ref \<Rightarrow> (refill list, 'z::state_ext) s_monad"
+where
+  "get_refills sc_ptr = do
     sc \<leftarrow> get_sched_context sc_ptr;
-    assert (0 < sc_budget sc);
-    sc' \<leftarrow> return $ sc\<lparr>sc_remaining := sc_budget sc\<rparr>;
+    return $ sc_refills sc
+  od"
+
+definition
+  refill_capacity :: "obj_ref \<Rightarrow> time \<Rightarrow> (time, 'z::state_ext) s_monad"
+where
+  "refill_capacity sc_ptr usage = do
+    refills \<leftarrow> get_refills sc_ptr;
+    return $ refills_capacity usage refills
+  od"
+
+definition
+  sufficient_refills :: "time \<Rightarrow> refill list \<Rightarrow> bool"
+where
+  "sufficient_refills usage refills = (MIN_BUDGET < refills_capacity usage refills)"
+
+definition
+  refill_sufficient :: "obj_ref \<Rightarrow> time \<Rightarrow> (bool, 'z::state_ext) s_monad"
+where
+  "refill_sufficient sc_ptr usage = do
+    refills \<leftarrow> get_refills sc_ptr;
+    return $ sufficient_refills usage refills
+  od"
+
+definition
+  refill_ready :: "obj_ref \<Rightarrow> (bool, 'z::state_ext) s_monad"
+where
+  "refill_ready sc_ptr = do
+    cur_time \<leftarrow> gets cur_time;
+    sc \<leftarrow> get_sched_context sc_ptr;
+    sc_time \<leftarrow> return $ r_time (refill_hd sc);
+    return $ sc_time \<le> cur_time + kernelWCET_ticks
+  od"
+
+definition
+  refill_size :: "obj_ref \<Rightarrow> (nat, 'z::state_ext) s_monad"
+where
+  "refill_size sc_ptr = do
+    refills \<leftarrow> get_refills sc_ptr;
+    return $ size refills
+  od"
+
+definition
+  refill_single :: "obj_ref \<Rightarrow> (bool, 'z::state_ext) s_monad"
+where
+  "refill_single sc_ptr = do
+    sz \<leftarrow> refill_size sc_ptr;
+    return (sz = 1)
+  od"
+
+definition
+  refills_sum :: "refill list \<Rightarrow> time"
+where
+  "refills_sum rf = \<Sum> (set (map r_amount rf))"
+
+definition
+  refill_sum :: "obj_ref \<Rightarrow> (time, 'z::state_ext) s_monad"
+where
+  "refill_sum sc_ptr = do
+    refills \<leftarrow> get_refills sc_ptr;
+    return $ refills_sum refills
+  od"
+
+definition
+  set_refills :: "obj_ref \<Rightarrow> refill list \<Rightarrow> (unit, 'z::state_ext) s_monad"
+where
+  "set_refills sc_ptr refills = do
+    sc \<leftarrow> get_sched_context sc_ptr;
+    set_sched_context sc_ptr (sc\<lparr>sc_refills:= refills\<rparr>)
+  od"
+
+definition
+  refill_pop_head :: "obj_ref \<Rightarrow> (refill, 'z::state_ext) s_monad"
+where
+  "refill_pop_head sc_ptr = do
+    refills \<leftarrow> get_refills sc_ptr;
+    assert (1 < size refills);
+    set_refills sc_ptr (tl refills);
+    return $ hd refills
+  od"
+
+definition
+  refill_add_tail :: "obj_ref \<Rightarrow> refill \<Rightarrow> (unit, 'z::state_ext) s_monad"
+where
+  "refill_add_tail sc_ptr rfl = do
+    assert (r_amount rfl \<noteq> 0);
+    sc \<leftarrow> get_sched_context sc_ptr;
+    refills \<leftarrow> return $ sc_refills sc;
+    assert (size refills < sc_refill_max sc);
+    set_refills sc_ptr (refills @ [rfl])
+  od"
+
+definition
+  refill_new :: "obj_ref \<Rightarrow> nat \<Rightarrow> ticks \<Rightarrow> ticks \<Rightarrow> (unit, 'z::state_ext) s_monad"
+where
+  "refill_new sc_ptr max_refills budget period = do
+    sc \<leftarrow> get_sched_context sc_ptr;
+    assert (MIN_BUDGET < budget);
+    cur_time \<leftarrow> gets cur_time;
+    refill \<leftarrow> return \<lparr> r_time = cur_time, r_amount = budget \<rparr>;
+    sc' \<leftarrow> return $ sc\<lparr> sc_period := period, sc_refills := [refill], sc_refill_max := max_refills \<rparr>;
     set_sched_context sc_ptr sc'
+  od"
+
+
+definition
+  merge_refill :: "refill \<Rightarrow> refill \<Rightarrow> refill"
+where
+  "merge_refill r1 r2 = \<lparr> r_time = r_time r1, r_amount = r_amount r2 + r_amount r1 \<rparr>"
+
+definition
+  "can_merge_refill r1 r2 \<equiv> r_time r2 \<le> r_time r1 + r_amount r1"
+
+fun
+  refills_merge_prefix :: "refill list \<Rightarrow> refill list"
+where
+  "refills_merge_prefix [] = []"
+| "refills_merge_prefix [r] = [r]"
+| "refills_merge_prefix (r1 # r2 # rs) = 
+     (if can_merge_refill r1 r2
+      then refills_merge_prefix (merge_refill r1 r2 # rs)
+      else r1 # r2 # rs)"
+
+definition
+  refill_unblock_check :: "obj_ref \<Rightarrow> (unit, 'z::state_ext) s_monad"
+where
+  "refill_unblock_check sc_ptr = do
+    ct \<leftarrow> gets cur_time;
+    refills \<leftarrow> get_refills sc_ptr;
+    refills' \<leftarrow> return $ refills_merge_prefix ((hd refills)\<lparr>r_time := ct\<rparr> # tl refills);
+    refills'' \<leftarrow> return (if sufficient_refills 0 refills' then refills' else
+      let
+        r1 = hd refills';
+        r2 = hd (tl refills');
+        rs = tl (tl refills')
+      in \<lparr> r_time = r_time r2, r_amount = r_amount r2 + r_amount r1 \<rparr> # rs);
+    set_refills sc_ptr refills''
+  od"
+
+function
+  refills_budget_check :: "ticks \<Rightarrow> ticks \<Rightarrow> refill list \<Rightarrow> ticks \<times> refill list"
+where
+  "refills_budget_check period usage [] = (usage, [])"
+| "refills_budget_check period usage (r#rs) = (if r_amount r \<le> usage \<and> 0 < r_amount r
+     then refills_budget_check period (usage - r_amount r) (rs @ [r\<lparr>r_time := r_time r + period\<rparr>]) 
+     else (usage, r#rs))"
+  by pat_completeness auto
+
+termination refills_budget_check
+  apply (relation "measure (\<lambda>(p,u,rs). unat u)")
+   apply clarsimp
+  apply unat_arith
+  done
+
+definition
+  refill_budget_check :: "obj_ref \<Rightarrow> ticks \<Rightarrow> (ticks, 'z::state_ext) s_monad"
+where
+  "refill_budget_check sc_ptr usage = do    
+    sc \<leftarrow> get_sched_context sc_ptr;
+    period \<leftarrow> return $ sc_period sc;
+    refills \<leftarrow> return $ sc_refills sc;
+    rfhd \<leftarrow> return $ hd refills;
+
+    (usage', refills') \<leftarrow> return $ refills_budget_check period usage refills;
+
+    refills'' \<leftarrow> return (if 0 < usage' \<and> 0 < period then
+      let r1 = hd refills'; 
+          r1' = r1 \<lparr>r_time := r_time r1 + usage\<rparr>;
+          rs = tl refills'
+      in if rs \<noteq> [] \<and> can_merge_refill r1' (hd rs) then merge_refill r1' (hd rs) # tl rs else [r1]
+    else refills');
+
+    set_refills sc_ptr refills';
+
+    return usage'
+  od"
+
+definition
+  refill_split_check :: "obj_ref \<Rightarrow> time \<Rightarrow> (unit, 'z::state_ext) s_monad"
+where
+  "refill_split_check sc_ptr usage = do
+    ct \<leftarrow> gets cur_time;
+    sc \<leftarrow> get_sched_context sc_ptr;
+    refills \<leftarrow> return $ sc_refills sc;
+    rfhd \<leftarrow> return $ hd refills;
+    assert (0 < usage \<and> usage \<le> r_amount rfhd);
+    assert (r_time rfhd \<le> ct);
+
+    remaining \<leftarrow> return $ r_amount rfhd - usage;
+    if remaining < MIN_BUDGET \<and> size refills = 1
+    then
+      set_refills sc_ptr [\<lparr> r_time = r_time rfhd + sc_period sc, r_amount = r_amount rfhd \<rparr>]
+    else do
+      if size refills = sc_refill_max sc \<or> remaining < MIN_BUDGET
+      then
+        let r2 = hd (tl refills); rs = tl (tl refills) in
+        set_refills sc_ptr (r2 \<lparr>r_amount := r_amount r2 + remaining\<rparr> # rs)
+      else
+        set_refills sc_ptr (rfhd\<lparr>r_amount := remaining\<rparr> # tl refills);
+      new \<leftarrow> return \<lparr> r_time = r_time rfhd + sc_period sc, r_amount = usage \<rparr>;
+      refill_add_tail sc_ptr new
+    od
+  od"
+
+
+definition
+  refill_update :: "obj_ref \<Rightarrow> ticks \<Rightarrow> ticks \<Rightarrow> nat \<Rightarrow> (unit, 'z::state_ext) s_monad"
+where
+  "refill_update sc_ptr new_period new_budget new_max_refills =
+    refill_new sc_ptr new_max_refills new_budget new_period
+    (* RT: may need to tweak this in the future *)
+  "
+
+definition
+  postpone :: "obj_ref \<Rightarrow> (unit, 'z::state_ext) s_monad"
+where
+  "postpone sc_ptr = do
+    sc \<leftarrow> get_sched_context sc_ptr;
+    tcb_ptr \<leftarrow> assert_opt $ sc_tcb sc;
+    do_extended_op $ tcb_sched_action tcb_sched_dequeue tcb_ptr;
+    do_extended_op $ tcb_release_enqueue tcb_ptr;
+    modify (\<lambda>s. s\<lparr> reprogram_timer := True \<rparr>)
   od"
 
 text \<open>
@@ -33,15 +295,20 @@ text \<open>
   is runnable and add it to the scheduling queue if required
 \<close> 
 definition
-  sched_context_resume :: "obj_ref \<Rightarrow> (unit, 'z::state_ext) s_monad"
+  sched_context_resume :: "obj_ref option \<Rightarrow> (unit, 'z::state_ext) s_monad"
 where
-  "sched_context_resume sc_ptr = do
+  "sched_context_resume sc_ptr_opt \<equiv> case sc_ptr_opt of None \<Rightarrow> return ()
+  | Some sc_ptr \<Rightarrow> do
      sc \<leftarrow> get_sched_context sc_ptr;
-     tptr \<leftarrow> return $ the $ sc_tcb sc;
-     ts \<leftarrow> thread_get tcb_state tptr;
-     when (runnable ts \<and> 0 < sc_budget sc) $ do
-        recharge sc_ptr;
-        do_extended_op $ possible_switch_to tptr
+     tptr \<leftarrow> assert_opt $ sc_tcb sc;
+     in_release_q \<leftarrow> select_ext (in_release_queue tptr) {True,False};
+     sched \<leftarrow> is_schedulable tptr in_release_q;
+     when sched $ do
+       refill_unblock_check sc_ptr;
+       ts \<leftarrow> thread_get tcb_state tptr;
+       ready \<leftarrow> refill_ready sc_ptr;
+       sufficient \<leftarrow> refill_sufficient sc_ptr 0;
+       when (runnable ts \<and> 0 < sc_refill_max sc \<and> \<not>(ready \<and> sufficient)) $ postpone sc_ptr
     od
   od"
 
@@ -54,7 +321,7 @@ where
     sc \<leftarrow> get_sched_context sc_ptr;
     set_sched_context sc_ptr (sc\<lparr>sc_tcb := Some tcb_ptr\<rparr>);
     thread_set (\<lambda>tcb. tcb\<lparr>tcb_sched_context := Some sc_ptr\<rparr>) tcb_ptr; 
-    sched_context_resume sc_ptr
+    sched_context_resume (Some sc_ptr)
   od"
 
 
@@ -67,8 +334,9 @@ definition
 where
   "sched_context_unbind sc_ptr = do
      sc \<leftarrow> get_sched_context sc_ptr;
-     tptr \<leftarrow> return $ the $ sc_tcb sc;
+     tptr \<leftarrow> assert_opt $ sc_tcb sc;
      do_extended_op $ tcb_sched_action tcb_sched_dequeue tptr;
+     do_extended_op $ tcb_release_remove tptr;
      thread_set (\<lambda>tcb. tcb \<lparr> tcb_sched_context := None \<rparr>) tptr;
      cur \<leftarrow> gets $ cur_thread;
      when (tptr = cur) $ do_extended_op reschedule_required
@@ -108,46 +376,37 @@ definition
   invoke_sched_control_configure :: "sched_control_invocation \<Rightarrow> (unit, 'z::state_ext) se_monad"
 where
   "invoke_sched_control_configure iv \<equiv>
-  case iv of InvokeSchedControlConfigure sc_ptr budget \<Rightarrow> liftE $ do
+  case iv of InvokeSchedControlConfigure sc_ptr budget period mrefills \<Rightarrow> liftE $ do
     sc \<leftarrow> get_sched_context sc_ptr;
-    set_sched_context sc_ptr (sc\<lparr>sc_budget:= budget\<rparr>);
-    recharge sc_ptr;
+    period \<leftarrow> return (if budget = period then 0 else period);
     when (sc_tcb sc \<noteq> None) $ do
-      tcb_ptr \<leftarrow> return $ the (sc_tcb sc);
-      tcb \<leftarrow> thread_get id tcb_ptr;
-      do_extended_op $ schedule_tcb tcb_ptr tcb;
-      if \<not>schedulable tcb then
-        do_extended_op $ tcb_sched_action tcb_sched_dequeue tcb_ptr
+      tcb_ptr \<leftarrow> assert_opt $ sc_tcb sc;
+      do_extended_op $ tcb_release_remove tcb_ptr;
+      st \<leftarrow> get_thread_state tcb_ptr;
+      if 0 < sc_refill_max sc \<and> runnable st then do
+        refill_update sc_ptr period budget mrefills;
+        sched_context_resume (Some sc_ptr)
+      od
       else
-        do_extended_op $ possible_switch_to tcb_ptr
+        refill_new sc_ptr mrefills budget period
     od
   od"
 
 
-text \<open> Update time consumption of given scheduling context and current domain. \<close>
+text \<open> Update time consumption of current scheduling context and current domain. \<close>
 definition
-  commit_time :: "obj_ref \<Rightarrow> (unit, 'z::state_ext) s_monad"
+  commit_time :: "(unit, 'z::state_ext) s_monad"
 where
-  "commit_time sc_ptr = do
-    sc \<leftarrow> get_sched_context sc_ptr;
+  "commit_time = do
     consumed \<leftarrow> gets consumed_time;
-    rem' \<leftarrow> return (if sc_remaining sc < consumed then 0 else sc_remaining sc - consumed);
-    set_sched_context sc_ptr (sc\<lparr>sc_remaining := rem'\<rparr>);
+    ct \<leftarrow> gets cur_thread;
+    it \<leftarrow> gets idle_thread;
+    when (0 < consumed \<and> ct \<noteq> it) $ do
+      csc \<leftarrow> gets_the cur_sc;
+      refill_split_check csc consumed
+    od;
     do_extended_op $ commit_domain_time;
-    modify (\<lambda>s. s\<lparr>cur_time := cur_time s + consumed \<rparr>);
     modify (\<lambda>s. s\<lparr>consumed_time := 0\<rparr> )
-  od"
-
-definition
-  is_cur_thread_expired :: "(bool,'z::state_ext) s_monad"
-where
-  "is_cur_thread_expired = do
-     cur \<leftarrow> gets cur_thread;
-     tcb \<leftarrow> gets_the $ get_tcb cur;
-     sc_ptr \<leftarrow> return (the (tcb_sched_context tcb));
-     sc \<leftarrow> get_sched_context sc_ptr;
-     consumed \<leftarrow> gets consumed_time;
-     return (sc_remaining sc < consumed + kernelWCET_ticks)
   od"
 
 
